

$$\frac{\partial C}{\partial b_j^l} = \delta_j^l \quad \text{Rate of change of the cost with respect to any bias in the network?}$$

Take the left hand side,

$$\begin{aligned} \frac{\partial C}{\partial b_j^l} &= \frac{\partial C}{\partial z_j^l} \frac{\partial z_j^l}{\partial b_j^l} = \frac{\partial C}{\partial z_j^l} \frac{\partial}{\partial b_j^l} \left(\sum_k w_{jk}^l a_k^{l-1} + b_j^l \right) \\ &= \frac{\partial C}{\partial z_j^l} \cdot (0 + 1) \end{aligned}$$

$$\frac{\partial C}{\partial b_j^l} = \delta_j^l$$

(From equation 29)

Rate of change of the cost with respect to any weight in the network:

$$\frac{\partial C}{\partial w_{jk}^l} = a_k^{l-1} \delta_j^l$$

Proof:

Take the left hand side

$$\frac{\partial C}{\partial w_{jk}^l} = \frac{\partial C}{\partial z_j^l} \frac{\partial z_j^l}{\partial w_{jk}^l}$$

$$= \delta_j^l \cdot \frac{\partial}{\partial w_{jk}^l} \sum_k w_{jk}^l a_k^{l-1} + b_j^l$$

$$\frac{\partial C}{\partial w_{jk}^l} = \delta_j^l \cdot a_k^{l-1}$$